SStructTT/SStruct/Static/Context.lean
@@ -1,12 +1,17 @@
 import SStructTT.SStruct.Syntax
 
 namespace SStruct.Static
+variable {Srt : Type}
 abbrev Ctx Srt := List (Tm Srt)
 
 @[scoped aesop safe [constructors]]
-inductive Has {Srt} : Ctx Srt -> Var -> Tm Srt -> Prop where
+inductive Has : Ctx Srt -> Var -> Tm Srt -> Prop where
   | zero Γ A :
     Has (A :: Γ) 0 A.[shift 1]
   | succ Γ A B x :
     Has Γ x A ->
     Has (B :: Γ) (x + 1) A.[shift 1]
+
+lemma Has.var_lt_length {Γ : Ctx Srt} {x A} :
+    Has Γ x A -> x < Γ.length := by
+  intro hs; induction hs <;> aesop
